core/FuncSpec.v
@@ -1,0 +1,33 @@
+Require Import Coq.Lists.List.
+Require Import Poulet4.Typed.
+Require Import Poulet4.Syntax.
+Require Import Poulet4.Value.
+Require Import Poulet4.Semantics.
+Require Import ProD3.core.Coqlib.
+Require Import ProD3.core.Hoare.
+
+Section FuncSpec.
+
+Context {tags_t: Type} {tags_t_inhabitant : Inhabitant tags_t}.
+Notation Val := (@ValueBase bool).
+Notation Sval := (@ValueBase (option bool)).
+Notation Lval := (@ValueLvalue tags_t).
+
+Notation ident := (String.string).
+Notation path := (list ident).
+
+Context `{target : @Target tags_t (@Expression tags_t)}.
+
+Definition hoare_func_modifies (ge : genv) (p : path) (func : @fundef tags_t) (vars : list path) (exts : list path) :=
+  forall st inargs targs st' outargs sig,
+    exec_func ge read_ndetbit p st func targs inargs st' outargs sig ->
+    (forall q, ~(In q vars) -> PathMap.get q (get_memory st) = PathMap.get q (get_memory st'))
+    /\ (forall q, ~(In q exts) -> PathMap.get q (get_memory st) = PathMap.get q (get_memory st')).
+
+Definition hoare_func_spec (ge : genv) (p : path) (pre : arg_assertion)
+    (func : @fundef tags_t) (targs : list P4Type) (post : arg_ret_assertion)
+    (vars : list path) (exts : list path) :=
+  hoare_func ge p pre func targs post
+    /\ hoare_func_modifies ge p func vars exts.
+
+End FuncSpec.
