core/Tactics.v
@@ -1,0 +1,77 @@
+Require Import Poulet4.Typed.
+Require Import Poulet4.Syntax.
+Require Import Poulet4.Value.
+Require Import Poulet4.Semantics.
+Require Import ProD3.core.Hoare.
+Require Import ProD3.core.ConcreteHoare.
+Require Import ProD3.core.AssertionNotations.
+
+Ltac forward_builtin :=
+  lazymatch goal with
+  | |- hoare_call _ _ _ _ _ =>
+      (eapply hoare_call_builtin';
+        [ reflexivity (* is_no_dup *)
+        | reflexivity (* eval_lexpr *)
+        | reflexivity (* eval_args *)
+        | reflexivity (* eval_builtin *)
+        ])
+      || fail "Not a built-in function"
+  | _ =>
+      fail "Not a hoare_call"
+  end.
+
+Ltac forward_stmt :=
+  lazymatch goal with
+  | |- hoare_stmt _ _ (MEM _ (EXT _)) ?stmt _ =>
+      lazymatch stmt with
+      (* hoare_stmt_var_call' *)
+      | MkStatement _
+            (StatVariable _ _
+                (Some (MkExpression _ (ExpFunctionCall ?func _ _) _ _))
+                ?loc) _ =>
+          lazymatch loc with
+          | LInstance _ => idtac (* ok *)
+          | LGlobal _ => fail "Cannot declacre a variable with LGlobal locator"
+          | _ => fail "Unrecognized locator expression" loc
+          end;
+          eapply hoare_stmt_var_call';
+            [ reflexivity (* is_call_expression *)
+            | forward_builtin (* hoare_call *)
+            | reflexivity (* is_no_dup *)
+            | reflexivity (* eval_write *)
+            ]
+      (* hoare_stmt_assign_call' *)
+      | MkStatement _ (StatAssignment _ (MkExpression _ (ExpFunctionCall ?func _ _) _ _)) _ =>
+          eapply hoare_stmt_assign_call';
+            [ reflexivity (* is_call_expression *)
+            | reflexivity (* eval_lexpr *)
+            | forward_builtin (* hoare_call *)
+            | reflexivity (* is_no_dup *)
+            | reflexivity (* eval_write *)
+            ]
+      (* hoare_stmt_assign' *)
+      | MkStatement _ (StatAssignment _ _) _ =>
+          eapply hoare_stmt_assign';
+            [ reflexivity (* is_call_expression *)
+            | reflexivity (* is_no_dup *)
+            | reflexivity (* eval_lexpr *)
+            | reflexivity (* eval_expr *)
+            | reflexivity (* eval_write *)
+            ]
+      | _ =>
+          fail 0 stmt "is not supported"
+      end
+  | _ => fail "The goal is not in the form of (hoare_stmt _ _ (MEM _ (EXT _)) _ _)"
+  end.
+
+Ltac forward :=
+  lazymatch goal with
+  | |- hoare_block _ _ (MEM _ (EXT _)) ?block _ =>
+      lazymatch block with
+      | BlockEmpty _ => idtac (* TODO *)
+      | BlockCons _ _ =>
+          eapply hoare_block_cons;
+          only 1 : forward_stmt
+      end
+  | _ => fail "The goal is not in the form of (hoare_block _ _ (MEM _ (EXT _)) _ _)"
+  end.
